formal-proofs/theories/lib/thread_queue/callback.v
@@ -1,0 +1,193 @@
+From iris.heap_lang Require Import notation lang.
+From SegmentQueue.util Require Import cmra.
+
+From iris.base_logic Require Import lib.invariants.
+From iris.program_logic Require Import atomic.
+From iris.bi.lib Require Import fractional.
+From iris.heap_lang Require Import proofmode.
+From iris.algebra Require Import cmra excl csum auth csum numbers.
+
+Section proof.
+
+Inductive callback_state :=
+  | CallbackWaiting
+  | CallbackInvoked (v: val).
+
+Notation permit := (optionUR (csumR fracR (agreeR unitO))).
+
+Notation algebra := (authUR (prodUR
+                                  (* None: Waiting
+                                     Some: Invoked
+                                  *)
+                                  (optionUR (agreeR valO))
+                                  permit)).
+
+Class callbackG Σ := CallbackG {
+  callback_inG :> inG Σ algebra;
+}.
+Definition callbackΣ : gFunctors := #[GFunctor algebra].
+Instance subG_callbackΣ {Σ} : subG callbackΣ Σ -> callbackG Σ.
+Proof. solve_inG. Qed.
+
+Context `{heapG Σ} `{callbackG Σ} (N: namespace).
+
+(* true -> whole permit
+   false -> not present *)
+Definition permit_auth_ra (present: bool): permit :=
+  Some (if present then Cinl 1%Qp else Cinr (to_agree ())).
+
+(* true -> half the permit
+   false -> not present *)
+Definition permit_state_ra (present: bool): permit :=
+  Some (if present then Cinl (1 / 2)%Qp else Cinr (to_agree ())).
+
+Definition callback_auth_ra (p: leibnizO callback_state): algebra :=
+  ● match p with
+  | CallbackWaiting => (None, permit_auth_ra true)
+  | CallbackInvoked v => (Some (to_agree v), permit_auth_ra false)
+  end.
+
+Definition callback_invokation_permit (γ: gname) (q: Qp): iProp Σ :=
+  own γ (◯ (None, Some (Cinl q))).
+
+Definition callback_is_invoked (γ: gname) (v: val): iProp Σ :=
+  own γ (◯ (Some (to_agree v), permit_state_ra false)).
+
+Global Instance callback_invokation_permit_Timeless:
+  Timeless (callback_invokation_permit γ q).
+Proof. apply _. Qed.
+
+Global Instance callback_invokation_permit_Fractional γ:
+  Fractional (callback_invokation_permit γ).
+Proof.
+  iIntros (x y). rewrite /callback_invokation_permit.
+  by rewrite -own_op -auth_frag_op -!pair_op -Some_op -Cinl_op -frac_op'.
+Qed.
+
+Theorem callback_invokation_permit_valid γ q:
+  callback_invokation_permit γ q -∗ ⌜(q ≤ 1)%Qc⌝.
+Proof.
+  iIntros "HFuture". iDestruct (own_valid with "HFuture") as %HValid.
+  iPureIntro. move: HValid. rewrite auth_frag_valid. case=> _/=. 
+  rewrite Some_valid. by compute.
+Qed.
+
+Global Instance callback_is_invoked_Persistent:
+  Persistent (callback_is_invoked γ v).
+Proof. apply _. Qed.
+
+Theorem callback_invokation_permit_implies_not_invoked γ v q:
+  callback_invokation_permit γ q -∗ callback_is_invoked γ v -∗ False.
+Proof.
+  iIntros "H1 H2".
+  iDestruct (own_valid_2 with "H1 H2") as %[_ HValid]%pair_valid.
+  exfalso. move: HValid=> /=. by compute.
+Qed.
+
+Definition is_callback (P: val -> iProp Σ) (γk: gname) (k: val): iProp Σ :=
+  (⌜k ≠ #()⌝ ∗ (callback_invokation_permit γk 1%Qp -∗ ∀ v, P v -∗ WP (k v) {{_, True}})).
+
+(* Global Instance is_callback_persistent R γ k:
+  Persistent (is_callback R γ k).
+Proof. apply _. Qed. *)
+
+Instance callback_state_Inhabited: Inhabited callback_state.
+Proof. econstructor. econstructor. Qed.
+
+Lemma callback_is_invoked_from_auth_ra γ v:
+  own γ (callback_auth_ra (CallbackInvoked v)) ==∗
+  own γ (callback_auth_ra (CallbackInvoked v)) ∗ callback_is_invoked γ v.
+Proof.
+  iIntros "H●". iMod (own_update with "H●") as "[$ $]"; last done.
+  apply auth_update_core_id; first by apply _.
+  repeat (apply prod_included; split). all: simpl. all: try done.
+Qed.
+
+Theorem callback_invokation_permit_exclusive γ q:
+  callback_invokation_permit γ 1%Qp -∗ callback_invokation_permit γ q -∗ False.
+Proof.
+  iIntros "H1 H2". iCombine "H1" "H2" as "H".
+  iDestruct (own_valid with "H") as %HValid. exfalso. move: HValid.
+  case=> _/=.
+  move: (frac_valid' (1 + q)). case=> HOk _ HOk'. apply HOk in HOk'.
+  by eapply Qp_not_plus_q_ge_1.
+Qed.
+
+
+(* Theorem invokeCallback_spec P γ k (v: val):
+  is_callback P γ k -∗
+  {{{ ▷ P v ∗
+      callback_invokation_permit γ 1%Qp }}}
+    k v @ ⊤ ∖ ↑N
+  {{{ RET #(); callback_is_invoked γ v }}}.
+Proof.
+  iIntros "#HFuture". 
+  iInv "HFuture" as (p) "[>H● Hℓ]" "HInvClose". *)
+
+Theorem invokeCallback_spec P γ k (v: val):
+  {{{ is_callback P γ k ∗
+      ▷ P v ∗
+      callback_invokation_permit γ 1%Qp }}}
+    k v
+  {{{ r, RET #r; callback_is_invoked γ v }}}.
+Proof.
+Admitted.
+  (* iIntros (Φ) "((% & HIHCallback) & HP & HInvoke) HΦ".
+  rewrite /is_callback.
+  iApply "HCallback".
+
+
+
+  iIntros "#HFuture" (Φ) "AU". 
+  iInv "HFuture" as (p) "[>H● Hℓ]" "HInvClose".
+  iMod "AU" as "[[HR HPermit] [_ HClose]]".
+  destruct p.
+  - wp_cmpxchg_suc.
+    iMod (own_update_2 with "H● HPermit") as "[H● HCallbackInvoked]".
+    {
+      apply auth_update with
+          (a' := (Some (to_agree (Some v)),
+                  permit_auth_ra false, permit_auth_ra true)).
+      repeat apply prod_local_update'.
+      - by apply alloc_option_local_update.
+      - rewrite /permit_auth_ra.
+        etransitivity.
+        by apply delete_option_local_update, Cinl_exclusive, frac_full_exclusive.
+        by apply alloc_option_local_update.
+      - done.
+    }
+    iDestruct "HCallbackInvoked" as "#HCallbackInvoked".
+    iMod ("HClose" $! true with "HCallbackInvoked") as "HΦ".
+    iModIntro.
+    iMod ("HInvClose" with "[-HΦ]") as "_".
+    { iExists (CallbackInvoked v). iFrame.
+      iDestruct "HR" as "[$|HContra]".
+      destruct controlling_cancellation.
+      - iDestruct (callback_is_invoked_not_cancelled
+                     with "HCallbackInvoked HContra") as ">[]".
+      - iDestruct "HContra" as %[].
+    }
+    iModIntro. by wp_pures.
+  - iDestruct (own_valid_2 with "H● HPermit")
+      as %[[[_ HValid]%pair_included _]%pair_included _]%auth_both_valid.
+    exfalso. move: HValid. rewrite /permit_auth_ra.
+    rewrite Some_included. case=> HContra.
+    * inversion HContra.
+    * apply csum_included in HContra.
+      destruct HContra as
+          [HContra|[(? & ? & ? & HContra & ?)|(? & ? & HContra & ?)]];
+        simplify_eq.
+  - wp_cmpxchg_fail.
+    iMod (future_is_cancelled_from_auth_ra with "H●") as "[H● HFutureCancelled]".
+    destruct controlling_cancellation.
+    2: iDestruct "HR" as "[HR|%]"; last done.
+    all: iMod ("HClose" $! false with "[$]") as "HΦ"; iModIntro.
+    all: iMod ("HInvClose" with "[H● Hℓ]") as "_";
+      first by iExists FutureCancelled; iFrame.
+    all: iModIntro; by wp_pures.
+Qed. *)
+
+End proof.
+
+Typeclasses Opaque callback_invokation_permit 
+            callback_is_invoked is_callback.
